Superposition_Calculus/Superposition.thy
@@ -9,28 +9,24 @@ theory Superposition
     "Knuth_Bendix_Order.Subterm_and_Context"
 
     (* Theories from this formalization *)
+    "Multiset_Extra"
     "Abstract_Substitution_Extra_First_Order_Term"
+    "Unordered_Prod"
 begin
 
+no_notation subst_compose (infixl "\<circ>\<^sub>s" 75)
+no_notation subst_apply_term (infixl "\<cdot>" 67)
 
-section \<open>Wellfounded_Extra\<close>
+hide_type Inference_System.inference
+hide_const
+  Inference_System.Infer
+  Inference_System.prems_of
+  Inference_System.concl_of
+  Inference_System.main_prem_of
 
-definition lex_prodp where
-  "lex_prodp R\<^sub>A R\<^sub>B x y \<longleftrightarrow> R\<^sub>A (fst x) (fst y) \<or> fst x = fst y \<and> R\<^sub>B (snd x) (snd y)"
 
-lemma lex_prodp_lex_prod_iff[pred_set_conv]:
-  "lex_prodp R\<^sub>A R\<^sub>B x y \<longleftrightarrow> (x, y) \<in> lex_prod {(x, y). R\<^sub>A x y} {(x, y). R\<^sub>B x y}"
-  unfolding lex_prodp_def lex_prod_def by auto
-
-lemma lex_prod_lex_prodp_iff:
-  "lex_prod {(x, y). R\<^sub>A x y} {(x, y). R\<^sub>B x y} = {(x, y). lex_prodp R\<^sub>A R\<^sub>B x y}"
-  unfolding lex_prodp_def lex_prod_def by auto
-
-lemma transp_lex_prodp: "transp R\<^sub>A \<Longrightarrow> transp R\<^sub>B \<Longrightarrow> transp (lex_prodp R\<^sub>A R\<^sub>B)"
-  by (metis (full_types) lex_prodp_def transpD transpI)
-
-lemma wfP_lex_prodp: "wfP R\<^sub>A \<Longrightarrow> wfP R\<^sub>B \<Longrightarrow> wfP (lex_prodp R\<^sub>A R\<^sub>B)"
-  by (metis lex_prod_lex_prodp_iff wfP_def wf_lex_prod)
+lemma reflclp_iff: "\<And>R x y. R\<^sup>=\<^sup>= x y \<longleftrightarrow> R x y \<or> x = y"
+  by (metis sup2CI sup2E)
 
 
 section \<open>Abstract Substitutions\<close>
@@ -50,260 +46,740 @@ qed
 
 section \<open>First_Order_Terms And Abstract_Substitution\<close>
 
-no_notation subst_compose (infixl "\<circ>\<^sub>s" 75)
-no_notation subst_apply_term (infixl "\<cdot>" 67)
-
-type_synonym ('f, 'v) atom = "('f, 'v) term \<times> ('f, 'v) term"
-
-abbreviation subst_atm :: "('f, 'v) atom \<Rightarrow> ('f, 'v) subst \<Rightarrow> ('f, 'v) atom" where
-  "subst_atm A \<sigma> \<equiv> map_prod (\<lambda>t. subst_apply_term t \<sigma>) (\<lambda>t. subst_apply_term t \<sigma>) A"
-
-global_interpretation substitution_ops subst_atm Var subst_compose .
-
 notation subst_apply_term (infixl "\<cdot>t" 67)
-notation subst_atm_abbrev (infixl "\<cdot>a" 67)
-notation subst_lit (infixl "\<cdot>l" 67)
-notation subst_cls (infixl "\<cdot>" 67)
-notation comp_subst_abbrev (infixl "\<odot>" 67)
+notation subst_apply_ctxt (infixl "\<cdot>t\<^sub>c" 67)
+notation subst_compose (infixl "\<odot>" 75)
+
+type_synonym 't atom = "'t uprod"
+
+definition subst_atm ::
+  "('f, 'v) term atom \<Rightarrow> ('f, 'v) subst \<Rightarrow> ('f, 'v) term atom" (infixl "\<cdot>a" 67)
+where
+  "subst_atm A \<sigma> = map_uprod (\<lambda>t. subst_apply_term t \<sigma>) A"
+
+definition subst_lit ::
+  "('f, 'v) term atom literal \<Rightarrow> ('f, 'v) subst \<Rightarrow> ('f, 'v) term atom literal" (infixl "\<cdot>l" 67)
+where
+  "subst_lit L \<sigma> = map_literal (\<lambda>A. A \<cdot>a \<sigma>) L"
+
+definition subst_cls ::
+  "('f, 'v) term atom clause \<Rightarrow> ('f, 'v) subst \<Rightarrow> ('f, 'v) term atom clause" (infixl "\<cdot>" 67)
+where
+  "subst_cls C \<sigma> = image_mset (\<lambda>L. L \<cdot>l \<sigma>) C"
+
+definition vars_atm :: "('f, 'v) term atom \<Rightarrow> 'v set" where
+  "vars_atm p = (\<Union>t \<in> set_uprod p. vars_term t)"
+
+definition vars_lit :: "('f, 'v) term atom literal \<Rightarrow> 'v set" where
+  "vars_lit L = vars_atm (atm_of L)"
+
+definition vars_cls :: "('f, 'v) term atom clause \<Rightarrow> 'v set" where
+  "vars_cls C = (\<Union>L \<in> set_mset C. vars_lit L)"
+
+lemma vars_term_ctxt_apply_term[simp]: "vars_term c\<langle>t\<rangle> = vars_ctxt c \<union> vars_term t"
+  by (induction c) auto
+
+lemma vars_atm_make_uprod[simp]: "vars_atm (t\<^sub>1 \<approx> t\<^sub>2) = vars_term t\<^sub>1 \<union> vars_term t\<^sub>2"
+  by (simp add: vars_atm_def)
+
+lemma vars_lit_Pos[simp]: "vars_lit (Pos A) = vars_atm A"
+  by (simp add: vars_lit_def)
+
+lemma vars_lit_Neg[simp]: "vars_lit (Neg A) = vars_atm A"
+  by (simp add: vars_lit_def)
+
+lemma vars_cls_add_mset[simp]: "vars_cls (add_mset L C) = vars_lit L \<union> vars_cls C"
+  by (simp add: vars_cls_def)
+
+lemma vars_cls_plus[simp]: "vars_cls (C\<^sub>1 + C\<^sub>2) = vars_cls C\<^sub>1 \<union> vars_cls C\<^sub>2"
+  by (simp add: vars_cls_def)
+
+abbreviation is_ground_trm where
+  "is_ground_trm t \<equiv> vars_term t = {}"
+
+abbreviation is_ground_trm_ctxt where
+  "is_ground_trm_ctxt c \<equiv> vars_ctxt c = {}"
+
+abbreviation is_ground_atm where
+  "is_ground_atm A \<equiv> vars_atm A = {}"
+
+abbreviation is_ground_lit where
+  "is_ground_lit L \<equiv> vars_lit L = {}"
+
+abbreviation is_ground_cls where
+  "is_ground_cls C \<equiv> vars_cls C = {}"
+
+lemma subst_trm_ident_if_is_ground_trm[simp]: "is_ground_trm t \<Longrightarrow> t \<cdot>t \<sigma> = t"
+  by (simp add: subst_apply_term_ident)
+
+lemma subst_trm_ctxt_ident_if_is_ground_trm_ctxt[simp]: "is_ground_trm_ctxt c \<Longrightarrow> c \<cdot>t\<^sub>c \<sigma> = c"
+  by (induction c) (simp_all add: list.map_ident_strong)
+
+lemma subst_atm_ident_if_is_ground_atm[simp]: "is_ground_atm A \<Longrightarrow> A \<cdot>a \<sigma> = A"
+  by (simp add: subst_atm_def uprod.map_ident_strong vars_atm_def)
+
+lemma subst_lit_ident_if_is_ground_lit[simp]: "is_ground_lit L \<Longrightarrow> L \<cdot>l \<sigma> = L"
+  by (simp add: subst_lit_def literal.expand literal.map_sel(1) literal.map_sel(2) vars_lit_def)
+
+lemma subst_cls_ident_if_is_ground_cls[simp]: "is_ground_cls C \<Longrightarrow> C \<cdot> \<sigma> = C"
+  by (induction C) (simp_all add: subst_cls_def)
 
 
-interpretation substitution subst_atm Var subst_compose
-proof unfold_locales
-  show "\<And>A. A \<cdot>a Var = A"
-    by (simp add: prod.map_ident)
-next
-  show "\<And>A \<sigma> \<tau>. A \<cdot>a (\<sigma> \<odot> \<tau>) = A \<cdot>a \<sigma> \<cdot>a \<tau>"
-    by (simp add: prod.map_comp comp_def)
-next
-  show "\<And>\<sigma> \<tau>. (\<And>A. A \<cdot>a \<sigma> = A \<cdot>a \<tau>) \<Longrightarrow> \<sigma> = \<tau>"
-    by (rule subst_term_eqI) force
-next
-  fix C :: "('f, 'v) atom clause" and \<sigma> :: "('f, 'v) subst"
-  define T :: "('f, 'v) term set" where
-    "T = (\<Union>L \<in> set_mset C. {fst (atm_of L), snd (atm_of L)})"
-
-  assume ground_C_\<sigma>: "is_ground_cls (subst_cls C \<sigma>)"
-  have "term_subst.is_ground_set (term_subst.subst_set T \<sigma>)"
-    unfolding term_subst.is_ground_set_def
-  proof (rule ballI)
-    fix t' assume "t' \<in> term_subst.subst_set T \<sigma>"
-    then obtain t where "t \<in> T" and "t' = t \<cdot>t \<sigma>"
-      unfolding term_subst.subst_set_def by auto
-    then obtain L where "L \<in># C" and t_in: "t \<in> {fst (atm_of L), snd (atm_of L)}"
-      unfolding T_def by auto
-
-    from \<open>L \<in># C\<close> have "is_ground_lit (subst_lit L \<sigma>)"
-      using ground_C_\<sigma> is_ground_cls_def multi_member_split
-      by (metis (mono_tags, lifting) subst_cls_add_mset union_single_eq_member)
-    hence "is_ground_atm (subst_atm (atm_of L) \<sigma>)"
-      by (simp add: is_ground_lit_def)
-    then show "term_subst.is_ground t'"
-      unfolding \<open>t' = t \<cdot>t \<sigma>\<close>
-      using t_in
-      apply (cases "atm_of L")
-      apply simp_all
-      apply (simp add: is_ground_atm_def term_subst.is_ground_def)
-      using term_subst.is_ground_def is_ground_atm_def by force
-  qed
-  then obtain \<gamma> where
-    gr_\<gamma>: "term_subst.is_ground_subst \<gamma>" and
-    subst_\<gamma>_eq_subst_\<sigma>: "\<forall>x\<in>T. x \<cdot>t \<gamma> = x \<cdot>t \<sigma>"
-    using term_subst.make_ground_subst[of T \<sigma>] by auto
-
-  show "\<exists>\<gamma>. is_ground_subst \<gamma> \<and> subst_cls C \<gamma> = subst_cls C \<sigma>"
-  proof (intro exI conjI)
-    show "is_ground_subst \<gamma>"
-      using gr_\<gamma>
-      unfolding substitution_ops.is_ground_subst_def
-      by (smt (verit, best) prod.map_ident_strong prod.set_map imageE is_ground_atm_def
-          term_subst.is_ground_def term_subst.is_ground_subst_def)
-  next
-    show "subst_cls C \<gamma> = subst_cls C \<sigma>"
-    proof (rule subst_cls_cong)
-      fix L assume "L \<in># C"
-      then show "subst_atm (atm_of L) \<gamma> = subst_atm (atm_of L) \<sigma>"
-        using subst_\<gamma>_eq_subst_\<sigma>
-        by (cases "atm_of L") (auto simp: T_def)
-    qed
-  qed
+typedef ('f, 'v) gterm = \<open>{t :: ('f, 'v) term. is_ground_trm t}\<close>
+  morphisms term_gterm gterm_term
+proof -
+  have "is_ground_trm (Fun undefined [])"
+    by simp
+  thus "\<exists>x. x \<in> {t. is_ground_trm t}"
+    by blast
 qed
 
 
 section \<open>Superposition Calculus\<close>
 
-hide_type Inference_System.inference
-hide_const Inference_System.prems_of Inference_System.concl_of Inference_System.main_prem_of
-
 locale superposition_calculus =
-  fixes less_trm :: "('f, 'v) term \<Rightarrow> ('f, 'v) term \<Rightarrow> bool" (infix "\<prec>\<^sub>t" 50)
+  fixes
+    less_trm :: "('f, 'v) term \<Rightarrow> ('f, 'v) term \<Rightarrow> bool" (infix "\<prec>\<^sub>t" 50) and
+    select :: "('f, 'v) term atom clause \<Rightarrow> ('f, 'v) term atom clause"
   assumes
     transp_less_trm[simp]: "transp (\<prec>\<^sub>t)" and
-    wfP_less_trm[simp]: "wfP (\<prec>\<^sub>t)"
+    asymp_less_trm[simp]: "asymp (\<prec>\<^sub>t)" and
+    wfP_less_trm[simp]: "wfP (\<prec>\<^sub>t)" and
+    totalp_on_less_trm[simp]: "totalp_on {t. is_ground_trm t} (\<prec>\<^sub>t)" and
+    select_negative_lits: "\<And>C L. L \<in># select C \<Longrightarrow> is_neg L" and
+    select_stable_under_renaming: "\<And>C \<rho>. term_subst.is_renaming \<rho> \<Longrightarrow> select (C \<cdot> \<rho>) = select C \<cdot> \<rho>"
 begin
+
+lemma irreflp_less_trm[simp]: "irreflp (\<prec>\<^sub>t)"
+  by simp
 
 abbreviation lesseq_trm (infix "\<preceq>\<^sub>t" 50) where
   "lesseq_trm \<equiv> (\<prec>\<^sub>t)\<^sup>=\<^sup>="
 
-abbreviation less_atm :: "('f, 'v) atom \<Rightarrow> ('f, 'v) atom \<Rightarrow> bool" (infix "\<prec>\<^sub>a" 50) where
-  "less_atm \<equiv> lex_prodp (\<prec>\<^sub>t) (\<prec>\<^sub>t)"
+abbreviation less_atm :: "('f, 'v) term atom \<Rightarrow> ('f, 'v) term atom \<Rightarrow> bool" (infix "\<prec>\<^sub>a" 50) where
+  "less_atm A\<^sub>1 A\<^sub>2 \<equiv> multp (\<prec>\<^sub>t) (mset_uprod A\<^sub>1) (mset_uprod A\<^sub>2)"
 
 abbreviation lesseq_atm (infix "\<preceq>\<^sub>a" 50) where
   "lesseq_atm \<equiv> (\<prec>\<^sub>a)\<^sup>=\<^sup>="
 
-abbreviation less_lit :: "('f, 'v) atom literal \<Rightarrow> ('f, 'v) atom literal \<Rightarrow> bool" (infix "\<prec>\<^sub>l" 50) where
+abbreviation less_lit :: "('f, 'v) term atom literal \<Rightarrow> ('f, 'v) term atom literal \<Rightarrow> bool" (infix "\<prec>\<^sub>l" 50) where
   "less_lit \<equiv> Clausal_Logic.less_lit (\<prec>\<^sub>a)"
 
 abbreviation lesseq_lit (infix "\<preceq>\<^sub>l" 50) where
   "lesseq_lit \<equiv> (\<prec>\<^sub>l)\<^sup>=\<^sup>="
 
-abbreviation less_cls :: "('f, 'v) atom clause \<Rightarrow> ('f, 'v) atom clause \<Rightarrow> bool" (infix "\<prec>\<^sub>c" 50) where
+abbreviation less_cls :: "('f, 'v) term atom clause \<Rightarrow> ('f, 'v) term atom clause \<Rightarrow> bool" (infix "\<prec>\<^sub>c" 50) where
   "less_cls \<equiv> multp (\<prec>\<^sub>l)"
 
 abbreviation lesseq_cls (infix "\<preceq>\<^sub>c" 50) where
   "lesseq_cls \<equiv> (\<prec>\<^sub>c)\<^sup>=\<^sup>="
 
 
-section \<open>Rules\<close>
+lemma transp_less_atm[simp]: "transp (\<prec>\<^sub>a)"
+  using transp_less_trm transp_multp
+  by (metis (no_types, lifting) transpD transpI)
 
+lemma transp_less_lit[simp]: "transp (\<prec>\<^sub>l)"
+  by (simp add: transp_less_lit)
 
-inductive superposition ::
-  "('f, 'v) atom clause \<Rightarrow> ('f, 'v) atom clause \<Rightarrow> ('f, 'v) atom clause \<Rightarrow> bool"
-where
-  superpositionI: "
-    \<not> (P\<^sub>2 \<preceq>\<^sub>c P\<^sub>1) \<Longrightarrow>
-    P\<^sub>1 = add_mset L\<^sub>1 P\<^sub>1' \<Longrightarrow>
-    P\<^sub>2 = add_mset L\<^sub>2 P\<^sub>2' \<Longrightarrow>
-    (\<forall>L \<in># add_mset L\<^sub>1 P\<^sub>1'. \<not> (L\<^sub>1 \<preceq>\<^sub>l L)) \<Longrightarrow>
-    (\<forall>L \<in># add_mset L\<^sub>2 P\<^sub>2'. \<not> (L\<^sub>1 \<preceq>\<^sub>l L)) \<Longrightarrow>
-    \<P> \<in> {Pos, Neg} \<Longrightarrow>
-    L\<^sub>1 = \<P> (s\<^sub>1\<langle>u\<^sub>1\<rangle>, s\<^sub>1') \<or> L\<^sub>2 = \<P> (s\<^sub>1', s\<^sub>1\<langle>u\<rangle>) \<Longrightarrow>
-    L\<^sub>2 = Pos (t\<^sub>2, t\<^sub>2') \<or> L\<^sub>2 = Pos (t\<^sub>2', t\<^sub>2) \<Longrightarrow>
-    \<not> (s\<^sub>1\<langle>u\<^sub>1\<rangle> \<preceq>\<^sub>t s\<^sub>1') \<Longrightarrow>
-    \<not> (t\<^sub>2 \<preceq>\<^sub>t t\<^sub>2') \<Longrightarrow>
-    term_subst.is_imgu \<mu> {{u\<^sub>1, t\<^sub>2}} \<Longrightarrow>
-    C = add_mset (\<P> (s\<^sub>1\<langle>t\<^sub>2\<rangle>, s\<^sub>1')) (P\<^sub>1' + P\<^sub>2') \<cdot> \<mu> \<Longrightarrow>
-    superposition P\<^sub>1 P\<^sub>2 C"
+lemma transp_less_cls[simp]: "transp (\<prec>\<^sub>c)"
+  by (simp add: transp_multp)
 
-inductive eq_resolution :: "('f, 'v) atom clause \<Rightarrow> ('f, 'v) atom clause \<Rightarrow> bool" where
-  eq_resolutionI: "
-    P = add_mset L P' \<Longrightarrow>
-    L = Neg (t\<^sub>1, t\<^sub>2) \<Longrightarrow>
-    term_subst.is_imgu \<mu> {{t\<^sub>1, t\<^sub>2}} \<Longrightarrow>
-    C = P' \<cdot> \<mu> \<Longrightarrow>
-    eq_resolution P C"
+lemma totalp_on_less_atm[simp]: "totalp_on {A. is_ground_atm A} (\<prec>\<^sub>a)"
+proof (rule totalp_onI, unfold mem_Collect_eq)
+  fix A1 A2 :: "('f, 'v) Term.term uprod"
+  assume "is_ground_atm A1" and "is_ground_atm A2" and "A1 \<noteq> A2"
 
-inductive eq_factoring :: "('f, 'v) atom clause \<Rightarrow> ('f, 'v) atom clause \<Rightarrow> bool" where
-  eq_factoringI: "
-    P = add_mset L\<^sub>1 (add_mset L\<^sub>2 P') \<Longrightarrow>
-    (\<forall>L \<in># add_mset L\<^sub>2 P'. \<not> (L\<^sub>1 \<prec>\<^sub>l L)) \<Longrightarrow>
-    L\<^sub>1 = Pos (s\<^sub>1, t\<^sub>1) \<or> L\<^sub>1 = Pos (t\<^sub>1, s\<^sub>1) \<Longrightarrow>
-    L\<^sub>2 = Pos (s\<^sub>2, t\<^sub>2) \<or> L\<^sub>2 = Pos (t\<^sub>2, s\<^sub>2) \<Longrightarrow>
-    \<not> (s\<^sub>1 \<preceq>\<^sub>t t\<^sub>1) \<Longrightarrow>
-    \<not> (s\<^sub>2 \<preceq>\<^sub>t t\<^sub>2) \<Longrightarrow>
-    term_subst.is_imgu \<mu> {{s\<^sub>1, s\<^sub>2}} \<Longrightarrow>
-    C = add_mset (Pos (s\<^sub>1, s\<^sub>2)) (add_mset (Neg (t\<^sub>1, t\<^sub>2)) P') \<cdot> \<mu> \<Longrightarrow>
-    eq_factoring P C"
+  let ?GT = "{T. \<forall>t \<in># T. is_ground_trm t}"
 
-
-section \<open>Correctness\<close>
-
-lemma eq_resolution_preserves_groundness:
-  assumes ground_P: "is_ground_cls P" and step: "eq_resolution P C"
-  shows "is_ground_cls C"
-  using step
-proof (cases P C rule: eq_resolution.cases)
-  case (eq_resolutionI L P' t\<^sub>1 t\<^sub>2 \<mu>)
-  then show ?thesis
-    by (smt (verit, best) ground_P is_ground_cls_add_mset is_ground_subst_cls)
-qed
-
-lemma ground_correctness_eq_resolution:
-  assumes step: "eq_resolution P C" and ground_P: "is_ground_cls P"
-  shows "\<forall>I. refl I \<longrightarrow> I \<TTurnstile> P \<longrightarrow> I \<TTurnstile> C"
-  using step
-proof (cases P C rule: eq_resolution.cases)
-  case (eq_resolutionI L P' t\<^sub>1 t\<^sub>2 \<mu>)
-  with ground_P have "is_ground_atm (t\<^sub>1, t\<^sub>2)"
-    by (simp add: is_ground_cls_def is_ground_lit_def)
-  hence "term_subst.is_ground t\<^sub>1 \<and> term_subst.is_ground t\<^sub>2"
-    by (smt (verit, best) is_ground_subst_atm map_prod_simp prod.inject term_subst.is_ground_def)
-  hence "term_subst.is_ground_set {t\<^sub>1, t\<^sub>2}"
-    by (simp add: term_subst.is_ground_set_def)
-
-  moreover from \<open>term_subst.is_imgu \<mu> {{t\<^sub>1, t\<^sub>2}}\<close> have "term_subst.is_unifier \<mu> {t\<^sub>1, t\<^sub>2}"
-    by (simp add: term_subst.is_imgu_def term_subst.is_unifiers_def)
-
-  ultimately have "t\<^sub>1 = t\<^sub>2"
-    using term_subst.ball_eq_constant_if_unifier[of "{t\<^sub>2}" \<mu> t\<^sub>1]
-    by simp
-
-  show ?thesis
-  proof (intro allI impI)
-    fix I
-    assume "refl I" and "I \<TTurnstile> P"
-    then obtain K where "K \<in># P" and "I \<TTurnstile>l K"
-      by (auto simp: true_cls_def)
-    hence "K \<noteq> L"
-      by (metis \<open>refl I\<close> \<open>t\<^sub>1 = t\<^sub>2\<close> \<open>L = Neg (t\<^sub>1, t\<^sub>2)\<close> reflD true_lit_simps(2))
-    hence "K \<in># P'"
-      using \<open>K \<in># P\<close> \<open>P = add_mset L P'\<close>
-      by simp
-    hence "K \<in># P' \<cdot> \<mu>"
-      by (smt (verit, best) ground_P is_ground_cls_add_mset is_ground_subst_cls eq_resolutionI(1))
-    thus "I \<TTurnstile> C"
-      using \<open>C = P' \<cdot> \<mu>\<close> \<open>I \<TTurnstile>l K\<close>
-      by blast
+  show "A1 \<prec>\<^sub>a A2 \<or> A2 \<prec>\<^sub>a A1"
+  proof (rule totalp_on_multp[OF totalp_on_less_trm transp_less_trm, THEN totalp_onD])
+    show "\<And>M. M \<in> ?GT \<Longrightarrow> set_mset M \<subseteq> {t. is_ground_trm t}"
+      by auto
+  next
+    show "mset_uprod A1 \<in> ?GT"
+      using \<open>is_ground_atm A1\<close>
+      by (simp add: vars_atm_def set_uprod_def)
+  next
+    show "mset_uprod A2 \<in> ?GT"
+      using \<open>is_ground_atm A2\<close>
+      by (simp add: vars_atm_def set_uprod_def)
+  next
+    show "mset_uprod A1 \<noteq> mset_uprod A2"
+      using \<open>A1 \<noteq> A2\<close>
+      by (simp add: mset_uprod_inject)
   qed
 qed
 
-lemma ground_correctness_eq_factoring:
+lemma totalp_on_less_lit[simp]: "totalp_on {L. is_ground_lit L} (\<prec>\<^sub>l)"
+  using totalp_on_less_atm
+  by (smt (verit, del_insts) Neg_atm_of_iff le_boolE less_lit_def linorder_not_less
+      literal.collapse(1) mem_Collect_eq totalp_on_def vars_lit_def)
+
+lemma totalp_on_less_cls[simp]: "totalp_on {C. is_ground_cls C} (\<prec>\<^sub>c)"
+proof (rule totalp_on_multp)
+  show "totalp_on {L. is_ground_lit L} (\<prec>\<^sub>l)"
+    by simp
+next
+  show "transp (\<prec>\<^sub>l)"
+    by simp
+next
+  show "\<And>M. M \<in> {C. is_ground_cls C} \<Longrightarrow> set_mset M \<subseteq> {L. is_ground_lit L}"
+    by (metis (mono_tags, lifting) insert_DiffM mem_Collect_eq subsetI sup_eq_bot_iff
+        vars_cls_add_mset)
+qed
+
+lemma mset_uprod_make_uprod[simp]: "mset_uprod (t\<^sub>1 \<approx> t\<^sub>2) = {#t\<^sub>1, t\<^sub>2#}"
+  using Abs_uprod_inverse[of "{#t\<^sub>1, t\<^sub>2#}", simplified]
+  by (simp add: make_uprod_def)
+
+lemma make_uprod_eq_make_uprod_iff: "t\<^sub>1 \<approx> s\<^sub>1 = t\<^sub>2 \<approx> s\<^sub>2 \<longleftrightarrow> t\<^sub>1 = t\<^sub>2 \<and> s\<^sub>1 = s\<^sub>2 \<or> t\<^sub>1 = s\<^sub>2 \<and> s\<^sub>1 = t\<^sub>2"
+  by (metis add_mset_eq_single add_mset_remove_trivial diff_union_swap2 insert_noteq_member
+      make_uprod_sym mset_uprod_make_uprod)
+
+lemma multp_subset_supersetI: "multp (\<prec>\<^sub>t) A B \<Longrightarrow> C \<subseteq># A \<Longrightarrow> B \<subseteq># D \<Longrightarrow> multp (\<prec>\<^sub>t) C D"
+  by (metis subset_implies_multp subset_mset.antisym_conv2 transpE transp_less_trm transp_multp)
+
+lemma multp_plus_plusI:
+  assumes "transp R" "multp R A B"
+  shows "multp R (A + A) (B + B)"
+  using multp_repeat_mset_repeat_msetI[OF \<open>transp R\<close> \<open>multp R A B\<close>, of 2]
+  by (simp add: numeral_Bit0)
+
+(* lemma
+  defines "lift \<equiv> \<lambda>L t\<^sub>1 s\<^sub>1. if is_pos L then {#t\<^sub>1, s\<^sub>1#} else {#t\<^sub>1, t\<^sub>1, s\<^sub>1, s\<^sub>1#}"
+  assumes "atm_of L\<^sub>1 = t\<^sub>1 \<approx> s\<^sub>1" and "atm_of L\<^sub>2 = t\<^sub>2 \<approx> s\<^sub>2"
+  shows "L\<^sub>1 \<prec>\<^sub>l L\<^sub>2 \<longleftrightarrow> multp (\<prec>\<^sub>t) (lift L\<^sub>1 t\<^sub>1 s\<^sub>1) (lift L\<^sub>2 t\<^sub>2 s\<^sub>2)"
+  unfolding lift_def
+  using assms(2,3)
+  apply (cases L\<^sub>1; cases L\<^sub>2)
+  apply simp_all
+  apply auto
+  apply (erule transp_multp[THEN transpD, OF transp_less_trm, of "{#t\<^sub>1, s\<^sub>1#}" "{#t\<^sub>2, s\<^sub>2#}" "{#t\<^sub>2, t\<^sub>2, s\<^sub>2, s\<^sub>2#}"])
+  apply (simp add: subset_implies_multp)
+  unfolding make_uprod_eq_make_uprod_iff
+  apply (auto intro: subset_implies_multp) []
+  defer
+  defer
+  apply (auto elim: multp_subset_supersetI) []
+  apply (drule multp_plus_plusI[OF transp_less_trm])
+  apply (simp add: add_mset_commute)
+  defer
+  apply simp
+  sledgehammer *)
+  
+  
+
+
+section \<open>Rules\<close>
+
+abbreviation is_maximal_lit where
+  "is_maximal_lit \<equiv> is_maximal_wrt (\<prec>\<^sub>l)"
+
+abbreviation is_strictly_maximal_lit where
+  "is_strictly_maximal_lit \<equiv> is_maximal_wrt (\<preceq>\<^sub>l)"
+
+inductive superposition ::
+  "('f, 'v) term atom clause \<Rightarrow> ('f, 'v) term atom clause \<Rightarrow> ('f, 'v) term atom clause \<Rightarrow> bool"
+where
+  superpositionI: "
+    term_subst.is_renaming \<rho>\<^sub>1 \<Longrightarrow>
+    term_subst.is_renaming \<rho>\<^sub>2 \<Longrightarrow>
+    vars_cls (P\<^sub>1 \<cdot> \<rho>\<^sub>1) \<inter> vars_cls (P\<^sub>2 \<cdot> \<rho>\<^sub>2) = {} \<Longrightarrow>
+    P\<^sub>1 = add_mset L\<^sub>1 P\<^sub>1' \<Longrightarrow>
+    P\<^sub>2 = add_mset L\<^sub>2 P\<^sub>2' \<Longrightarrow>
+    \<P> \<in> {Pos, Neg} \<Longrightarrow>
+    L\<^sub>1 = \<P> (s\<^sub>1\<langle>u\<^sub>1\<rangle> \<approx> s\<^sub>1') \<Longrightarrow>
+    L\<^sub>2 = Pos (t\<^sub>2 \<approx> t\<^sub>2') \<Longrightarrow>
+    \<not> is_Var u\<^sub>1 \<Longrightarrow>
+    term_subst.is_imgu \<mu> {{u\<^sub>1 \<cdot>t \<rho>\<^sub>1, t\<^sub>2 \<cdot>t \<rho>\<^sub>2}} \<Longrightarrow>
+    \<not> (P\<^sub>1 \<cdot> \<rho>\<^sub>1 \<cdot> \<mu> \<preceq>\<^sub>c P\<^sub>2 \<cdot> \<rho>\<^sub>2 \<cdot> \<mu>) \<Longrightarrow>
+    select P\<^sub>1 = {#} \<and> is_strictly_maximal_lit (L\<^sub>1 \<cdot>l \<rho>\<^sub>1 \<cdot>l \<mu>) (P\<^sub>1 \<cdot> \<rho>\<^sub>1 \<cdot> \<mu>) \<or> L\<^sub>1 \<in># select P\<^sub>1 \<Longrightarrow>
+    select P\<^sub>2 = {#} \<and> is_strictly_maximal_lit (L\<^sub>2 \<cdot>l \<rho>\<^sub>2 \<cdot>l \<mu>) (P\<^sub>2 \<cdot> \<rho>\<^sub>2 \<cdot> \<mu>) \<Longrightarrow>
+    \<not> (s\<^sub>1\<langle>u\<^sub>1\<rangle> \<cdot>t \<rho>\<^sub>1 \<cdot>t \<mu> \<preceq>\<^sub>t s\<^sub>1' \<cdot>t \<rho>\<^sub>1 \<cdot>t \<mu>) \<Longrightarrow>
+    \<not> (t\<^sub>2 \<cdot>t \<rho>\<^sub>2 \<cdot>t \<mu> \<preceq>\<^sub>t t\<^sub>2' \<cdot>t \<rho>\<^sub>2 \<cdot>t \<mu>) \<Longrightarrow>
+    C = add_mset (\<P> ((s\<^sub>1 \<cdot>t\<^sub>c \<rho>\<^sub>1)\<langle>t\<^sub>2 \<cdot>t \<rho>\<^sub>2\<rangle> \<approx> s\<^sub>1' \<cdot>t \<rho>\<^sub>1)) (P\<^sub>1' \<cdot> \<rho>\<^sub>1 + P\<^sub>2' \<cdot> \<rho>\<^sub>2) \<cdot> \<mu> \<Longrightarrow>
+    superposition P\<^sub>1 P\<^sub>2 C"
+
+inductive eq_resolution :: "('f, 'v) term atom clause \<Rightarrow> ('f, 'v) term atom clause \<Rightarrow> bool" where
+  eq_resolutionI: "
+    P = add_mset L P' \<Longrightarrow>
+    L = Neg (s\<^sub>1 \<approx> s\<^sub>2) \<Longrightarrow>
+    term_subst.is_imgu \<mu> {{s\<^sub>1, s\<^sub>2}} \<Longrightarrow>
+    select P = {#} \<and> is_maximal_lit (L \<cdot>l \<mu>) (P \<cdot> \<mu>) \<or> L \<in># select P \<Longrightarrow>
+    C = P' \<cdot> \<mu> \<Longrightarrow>
+    eq_resolution P C"
+
+inductive eq_factoring :: "('f, 'v) term atom clause \<Rightarrow> ('f, 'v) term atom clause \<Rightarrow> bool" where
+  eq_factoringI: "
+    P = add_mset L\<^sub>1 (add_mset L\<^sub>2 P') \<Longrightarrow>
+    L\<^sub>1 = Pos (s\<^sub>1 \<approx> s\<^sub>1') \<Longrightarrow>
+    L\<^sub>2 = Pos (t\<^sub>2 \<approx> t\<^sub>2') \<Longrightarrow>
+    select P = {#} \<and> is_maximal_lit (L\<^sub>1 \<cdot>l \<mu>) (P \<cdot> \<mu>) \<Longrightarrow>
+    \<not> (s\<^sub>1 \<cdot>t \<mu> \<preceq>\<^sub>t s\<^sub>1' \<cdot>t \<mu>) \<Longrightarrow>
+    term_subst.is_imgu \<mu> {{s\<^sub>1, t\<^sub>2}} \<Longrightarrow>
+    C = add_mset (Pos (s\<^sub>1 \<approx> t\<^sub>2')) (add_mset (Neg (s\<^sub>1' \<approx> t\<^sub>2')) P') \<cdot> \<mu> \<Longrightarrow>
+    eq_factoring P C"
+
+
+lemma subst_lit_Pos: "Pos A \<cdot>l \<sigma> = Pos (A \<cdot>a \<sigma>)"
+  by (simp add: subst_lit_def)
+
+lemma subst_lit_Neg: "Neg A \<cdot>l \<sigma> = Neg (A \<cdot>a \<sigma>)"
+  by (simp add: subst_lit_def)
+
+lemma subst_cls_add_mset: "add_mset L C \<cdot> \<sigma> = add_mset (L \<cdot>l \<sigma>) (C \<cdot> \<sigma>)"
+  by (simp add: subst_cls_def)
+
+lemma subst_cls_plus: "(C\<^sub>1 + C\<^sub>2) \<cdot> \<sigma> = (C\<^sub>1 \<cdot> \<sigma>) + (C\<^sub>2 \<cdot> \<sigma>)"
+  by (simp add: subst_cls_def)
+
+lemma superposition_preserves_groundness:
+  assumes
+    step: "superposition P1 P2 C" and
+    ground_P1: "is_ground_cls P1" and
+    ground_P2: "is_ground_cls P2"
+  shows "is_ground_cls C"
+  using step
+proof (cases P1 P2 C rule: superposition.cases)
+  case (superpositionI \<rho>\<^sub>1 \<rho>\<^sub>2 L\<^sub>1 P\<^sub>1' L\<^sub>2 P\<^sub>2' \<P> s\<^sub>1 u\<^sub>1 s\<^sub>1' t\<^sub>2 t\<^sub>2' \<mu>)
+  with ground_P1 ground_P2 have
+    "is_ground_cls P\<^sub>1'" and "is_ground_cls P\<^sub>2'" and
+    "is_ground_trm_ctxt s\<^sub>1" and "is_ground_trm u\<^sub>1" and "is_ground_trm s\<^sub>1'" and
+    "is_ground_trm t\<^sub>2" and "is_ground_trm t\<^sub>2'"
+    by auto
+  thus ?thesis
+    unfolding superpositionI
+    using \<open>\<P> \<in> {Pos, Neg}\<close>
+    by (auto simp: subst_cls_add_mset)
+qed
+
+lemma eq_resolution_preserves_groundness:
+  assumes step: "eq_resolution P C" and ground_P: "is_ground_cls P"
+  shows "is_ground_cls C"
+  using step
+proof (cases P C rule: eq_resolution.cases)
+  case (eq_resolutionI L P' s\<^sub>1 s\<^sub>2 \<mu>)
+  with ground_P have "is_ground_cls P'"
+    by (simp add: vars_cls_def)
+  thus ?thesis
+    unfolding eq_resolutionI by simp
+qed
+
+lemma eq_factoring_preserves_groundness:
   assumes step: "eq_factoring P C" and ground_P: "is_ground_cls P"
-  shows "\<forall>I. refl I \<longrightarrow> I \<TTurnstile> P \<longrightarrow> I \<TTurnstile> C"
+  shows "is_ground_cls C"
   using step
 proof (cases P C rule: eq_factoring.cases)
-  case (eq_factoringI L\<^sub>1 L\<^sub>2 P' s\<^sub>1 t\<^sub>1 s\<^sub>2 t\<^sub>2 \<mu>)
-  then show ?thesis
-    sorry
+  case (eq_factoringI L\<^sub>1 L\<^sub>2 P' s\<^sub>1 s\<^sub>1' t\<^sub>2 t\<^sub>2' \<mu>)
+  with ground_P have "is_ground_cls P'"
+    "is_ground_trm s\<^sub>1" "is_ground_trm s\<^sub>1'"
+    "is_ground_trm t\<^sub>2" "is_ground_trm t\<^sub>2'"
+    by simp_all
+  thus ?thesis
+    unfolding eq_factoringI by simp
 qed
 
 
 section \<open>Ground Layer\<close>
 
-abbreviation G_Inf :: "('f, 'v) atom clause inference set" where
-  "G_Inf \<equiv> {}"
+definition gcls_cls where
+  "gcls_cls \<equiv> map_clause (map_uprod gterm_term)"
 
-abbreviation G_Bot :: "('f, 'v) atom clause set" where
+definition cls_gcls where
+  "cls_gcls \<equiv> map_clause (map_uprod term_gterm)"
+
+lemma cls_gcls_empty_mset[simp]: "cls_gcls {#} = {#}"
+  by (simp add: cls_gcls_def)
+
+lemma cls_gcls_inverse[simp]: "gcls_cls (cls_gcls C) = C"
+  unfolding gcls_cls_def cls_gcls_def
+  by (simp add: multiset.map_comp literal.map_comp uprod.map_comp comp_def
+      literal.map_ident_strong term_gterm_inverse uprod.map_ident_strong)
+
+lemma is_ground_cls_gcls[simp]: "is_ground_cls (cls_gcls C)"
+  unfolding cls_gcls_def
+  apply (simp add: vars_cls_def vars_lit_def vars_atm_def)
+  by (smt (verit) imageE literal.map_sel(1) literal.map_sel(2) mem_Collect_eq term_gterm
+      uprod.set_map)
+
+lemma is_ground_lit_if_in_ground_cls[intro]:
+  "L \<in># C \<Longrightarrow> is_ground_cls C \<Longrightarrow> is_ground_lit L"
+  by (simp add: vars_cls_def)
+
+lemma is_ground_atm_if_in_ground_lit[intro]:
+  "A \<in> set_literal L \<Longrightarrow> is_ground_lit L \<Longrightarrow> is_ground_atm A"
+  by (metis literal.set_cases vars_lit_Neg vars_lit_Pos)
+
+lemma is_ground_term_if_in_ground_atm[intro]:
+  "t \<in> set_uprod A \<Longrightarrow> is_ground_atm A \<Longrightarrow> is_ground_trm t"
+  by (simp add: vars_atm_def)
+
+lemma gcls_cls_inverse[simp]: "is_ground_cls C \<Longrightarrow> cls_gcls (gcls_cls C) = C"
+  unfolding cls_gcls_def gcls_cls_def
+  by (auto simp: literal.map_comp uprod.map_comp comp_def
+      elim!: is_ground_term_if_in_ground_atm is_ground_atm_if_in_ground_lit is_ground_lit_if_in_ground_cls
+      intro!: multiset.map_ident_strong literal.map_ident_strong uprod.map_ident_strong gterm_term_inverse)
+
+definition G_Inf :: "('f, 'v) gterm atom clause inference set" where
+  "G_Inf \<equiv>
+    {Infer [P\<^sub>2, P\<^sub>1] (gcls_cls C) | P\<^sub>2 P\<^sub>1 C. superposition (cls_gcls P\<^sub>1) (cls_gcls P\<^sub>2) C} \<union>
+    {Infer [P] (gcls_cls C) | P C. eq_resolution (cls_gcls P) C} \<union>
+    {Infer [P] (gcls_cls C) | P C. eq_factoring (cls_gcls P) C}"
+
+abbreviation G_Bot :: "('f, 'v) gterm atom clause set" where
   "G_Bot \<equiv> {{#}}"
 
-abbreviation G_entails :: "('f, 'v) atom clause set \<Rightarrow> ('f, 'v) atom clause set \<Rightarrow> bool" where
-  "G_entails \<equiv> (\<TTurnstile>e)"
+definition compatible_with_Fun :: "(('f, 'v) Term.term \<times> ('f, 'v) Term.term) set \<Rightarrow> bool" where
+  "compatible_with_Fun I \<longleftrightarrow>
+    (\<forall>f ts ts'. list_all2 (\<lambda>t t'. (t, t') \<in> I) ts ts' \<longrightarrow> (Fun f ts, Fun f ts') \<in> I)"
+
+definition G_entails ::
+  "('f, 'v) gterm atom clause set \<Rightarrow> ('f, 'v) gterm atom clause set \<Rightarrow> bool"
+where
+  "G_entails N\<^sub>1 N\<^sub>2 \<longleftrightarrow> (\<forall>(I :: (('f, 'v) Term.term \<times> ('f, 'v) Term.term) set).
+    refl I \<longrightarrow> trans I \<longrightarrow> sym I \<longrightarrow> compatible_with_Fun I \<longrightarrow>
+    (\<lambda>(t\<^sub>1, t\<^sub>2). t\<^sub>1 \<approx> t\<^sub>2) ` I \<TTurnstile>s (cls_gcls ` N\<^sub>1) \<longrightarrow>
+    (\<lambda>(t\<^sub>1, t\<^sub>2). t\<^sub>1 \<approx> t\<^sub>2) ` I \<TTurnstile>s (cls_gcls ` N\<^sub>2))"
+
+
+subsection \<open>Correctness\<close>
+
+lemma true_lit_uprod_iff_true_lit_prod[simp]:
+  assumes "sym I"
+  shows
+    "(\<lambda>(t\<^sub>1, t\<^sub>2). t\<^sub>1 \<approx> t\<^sub>2) ` I \<TTurnstile>l Pos (t \<approx> t') \<longleftrightarrow> I \<TTurnstile>l Pos (t, t')"
+    "(\<lambda>(t\<^sub>1, t\<^sub>2). t\<^sub>1 \<approx> t\<^sub>2) ` I \<TTurnstile>l Neg (t \<approx> t') \<longleftrightarrow> I \<TTurnstile>l Neg (t, t')"
+  unfolding true_lit_simps atomize_conj
+  using \<open>sym I\<close>[THEN symD]
+  by (smt (z3) case_prod_unfold image_iff make_uprod_eq_make_uprod_iff pair_imageI prod.collapse)
+
+lemma correctness_ground_superposition:
+  assumes step: "superposition P1 P2 C" and ground_P1: "is_ground_cls P1" and ground_P2: "is_ground_cls P2"
+  shows "G_entails {gcls_cls P1, gcls_cls P2} {gcls_cls C}"
+  using step
+proof (cases P1 P2 C rule: superposition.cases)
+  case (superpositionI \<rho>\<^sub>1 \<rho>\<^sub>2 L\<^sub>1 P\<^sub>1' L\<^sub>2 P\<^sub>2' \<P> s\<^sub>1 u\<^sub>1 s\<^sub>1' t\<^sub>2 t\<^sub>2' \<mu>)
+  with ground_P1 ground_P2 have "is_ground_atm (s\<^sub>1\<langle>u\<^sub>1\<rangle> \<approx> s\<^sub>1')" and "is_ground_atm (t\<^sub>2 \<approx> t\<^sub>2')"
+    by (metis insert_iff singletonD sup_eq_bot_iff vars_cls_add_mset vars_lit_Neg vars_lit_Pos)+
+  hence
+    "is_ground_trm s\<^sub>1\<langle>u\<^sub>1\<rangle>" and "is_ground_trm_ctxt s\<^sub>1" and "is_ground_trm u\<^sub>1" and
+    "is_ground_trm s\<^sub>1'" and "is_ground_trm t\<^sub>2" and "is_ground_trm t\<^sub>2'"
+    by simp_all
+  hence "term_subst.is_ground_set {u\<^sub>1 \<cdot>t \<rho>\<^sub>1, t\<^sub>2 \<cdot>t \<rho>\<^sub>2}"
+    by (simp add: term_subst.is_ground_set_def term_subst.is_ground_def)
+  moreover have "term_subst.is_unifier \<mu> {u\<^sub>1 \<cdot>t \<rho>\<^sub>1, t\<^sub>2 \<cdot>t \<rho>\<^sub>2}"
+    using \<open>term_subst.is_imgu \<mu> {{u\<^sub>1 \<cdot>t \<rho>\<^sub>1, t\<^sub>2 \<cdot>t \<rho>\<^sub>2}}\<close>
+    by (simp add: term_subst.is_imgu_def term_subst.is_unifiers_def)
+  ultimately have "u\<^sub>1 = t\<^sub>2"
+    using term_subst.ball_eq_constant_if_unifier[of "{_}" \<mu>, simplified]
+    using \<open>is_ground_trm t\<^sub>2\<close> \<open>is_ground_trm u\<^sub>1\<close> by auto
+
+  have 1: "cls_gcls ` {gcls_cls P1, gcls_cls P2} = {P1, P2}"
+    using ground_P1 ground_P2 by simp_all
+
+  have 2: "cls_gcls ` {gcls_cls C} = {C}"
+    using superposition_preserves_groundness[OF step ground_P1 ground_P2] by simp
+
+  show ?thesis
+    unfolding G_entails_def 1 2 true_clss_singleton
+    unfolding true_clss_insert
+  proof (intro allI impI, elim conjE)
+    fix I :: "(('f, 'v) Term.term \<times> ('f, 'v) Term.term) set"
+
+    let ?I' = "(\<lambda>(t\<^sub>1, t\<^sub>2). t\<^sub>1 \<approx> t\<^sub>2) ` I"
+
+    assume "refl I" and "trans I" and "sym I" and "compatible_with_Fun I" and
+      "?I' \<TTurnstile> P1" and "?I' \<TTurnstile> P2"
+    then obtain K1 K2 :: "('f, 'v) Term.term uprod literal" where
+      "K1 \<in># P1" and "?I' \<TTurnstile>l K1" and "K2 \<in># P2" and "?I' \<TTurnstile>l K2"
+      by (auto simp: true_cls_def)
+
+    show "?I' \<TTurnstile> C"
+    proof (cases "K1 = \<P> (s\<^sub>1\<langle>u\<^sub>1\<rangle> \<approx> s\<^sub>1')")
+      case True
+      then show ?thesis
+        using ground_P1 ground_P2 \<open>?I' \<TTurnstile>l K1\<close>
+        unfolding superpositionI \<open>u\<^sub>1 = t\<^sub>2\<close>
+        using \<open>is_ground_trm_ctxt s\<^sub>1\<close> \<open>is_ground_trm s\<^sub>1'\<close> \<open>is_ground_trm t\<^sub>2\<close> by auto
+    next
+      case False
+      hence "K1 \<in># P\<^sub>1'"
+        using \<open>K1 \<in># P1\<close>
+        unfolding superpositionI by simp
+      hence "?I' \<TTurnstile> P\<^sub>1'"
+        using \<open>?I' \<TTurnstile>l K1\<close> by blast
+      moreover have "\<And>\<sigma>. P\<^sub>1' \<cdot> \<sigma> = P\<^sub>1'"
+        using ground_P1
+        unfolding superpositionI by force
+      ultimately show ?thesis
+        unfolding superpositionI
+        by (simp add: subst_cls_add_mset subst_cls_plus)
+    qed
+  qed
+qed
+
+lemma correctness_ground_eq_resolution:
+  assumes step: "eq_resolution P C" and ground_P: "is_ground_cls P"
+  shows "G_entails {gcls_cls P} {gcls_cls C}"
+  using step
+proof (cases P C rule: eq_resolution.cases)
+  case (eq_resolutionI L P' t\<^sub>1 t\<^sub>2 \<mu>)
+  with ground_P have "is_ground_atm (t\<^sub>1 \<approx> t\<^sub>2)"
+    by simp
+  hence "is_ground_trm t\<^sub>1" and "is_ground_trm t\<^sub>2"
+    by simp_all
+  hence "term_subst.is_ground_set {t\<^sub>1, t\<^sub>2}"
+    by (simp add: term_subst.is_ground_set_def term_subst.is_ground_def)
+
+  moreover from \<open>term_subst.is_imgu \<mu> {{t\<^sub>1, t\<^sub>2}}\<close> have "term_subst.is_unifier \<mu> {t\<^sub>1, t\<^sub>2}"
+    by (simp add: term_subst.is_imgu_def term_subst.is_unifiers_def)
+
+  ultimately have "t\<^sub>1 = t\<^sub>2"
+    using term_subst.ball_eq_constant_if_unifier[of "{t\<^sub>2}" \<mu> t\<^sub>1] by simp
+
+  have 1: "cls_gcls ` {gcls_cls P} = {P}"
+    using ground_P by simp
+
+  have 2: "cls_gcls ` {gcls_cls C} = {C}"
+    using eq_resolution_preserves_groundness[OF step ground_P] by simp
+
+  show ?thesis
+    unfolding G_entails_def 1 2 true_clss_singleton
+  proof (intro allI impI)
+    fix I
+    assume "refl I" and "(\<lambda>(t\<^sub>1, t\<^sub>2). t\<^sub>1 \<approx> t\<^sub>2) ` I \<TTurnstile> P"
+    then obtain K where "K \<in># P" and "(\<lambda>(t\<^sub>1, t\<^sub>2). t\<^sub>1 \<approx> t\<^sub>2) ` I \<TTurnstile>l K"
+      by (auto simp: true_cls_def)
+    hence "K \<noteq> L"
+      by (metis \<open>refl I\<close> \<open>t\<^sub>1 = t\<^sub>2\<close> local.eq_resolutionI(2) pair_imageI reflD true_lit_simps(2))
+    hence "K \<in># P'"
+      using \<open>K \<in># P\<close> \<open>P = add_mset L P'\<close> by simp
+    hence "K \<in># P' \<cdot> \<mu>"
+      using ground_P eq_resolutionI(1) by fastforce
+    thus "(\<lambda>(t\<^sub>1, t\<^sub>2). t\<^sub>1 \<approx> t\<^sub>2) ` I \<TTurnstile> C"
+      using \<open>C = P' \<cdot> \<mu>\<close> \<open>(\<lambda>(t\<^sub>1, t\<^sub>2). t\<^sub>1 \<approx> t\<^sub>2) ` I \<TTurnstile>l K\<close> by blast
+  qed
+qed
+
+lemma correctness_ground_eq_factoring:
+  assumes step: "eq_factoring P C" and ground_P: "is_ground_cls P"
+  shows "G_entails {gcls_cls P} {gcls_cls C}"
+  using step
+proof (cases P C rule: eq_factoring.cases)
+  case (eq_factoringI L\<^sub>1 L\<^sub>2 P' s\<^sub>1 s\<^sub>1' t\<^sub>2 t\<^sub>2' \<mu>)
+  with ground_P have "is_ground_atm (s\<^sub>1 \<approx> s\<^sub>1')" and "is_ground_atm (t\<^sub>2 \<approx> t\<^sub>2')"
+    by simp_all
+  hence "is_ground_trm s\<^sub>1" and "is_ground_trm s\<^sub>1'" and "is_ground_trm t\<^sub>2" and "is_ground_trm t\<^sub>2'"
+    by simp_all
+  hence "term_subst.is_ground_set {s\<^sub>1, t\<^sub>2}"
+    by (simp add: term_subst.is_ground_set_def term_subst.is_ground_def)
+  moreover from \<open>term_subst.is_imgu \<mu> {{s\<^sub>1, t\<^sub>2}}\<close> have "term_subst.is_unifier \<mu> {s\<^sub>1, t\<^sub>2}"
+    by (simp add: term_subst.is_imgu_def term_subst.is_unifiers_def)
+  ultimately have "s\<^sub>1 = t\<^sub>2"
+    using term_subst.ball_eq_constant_if_unifier[of "{t\<^sub>2}" \<mu> s\<^sub>1] by simp
+
+  have 1: "cls_gcls ` {gcls_cls P} = {P}"
+    using ground_P by simp
+
+  have 2: "cls_gcls ` {gcls_cls C} = {C}"
+    using eq_factoring_preserves_groundness[OF step ground_P] by simp
+
+  show ?thesis
+    unfolding G_entails_def 1 2 true_clss_singleton
+  proof (intro allI impI)
+    fix I :: "(('f, 'v) Term.term \<times> ('f, 'v) Term.term) set"
+
+    let ?I' = "(\<lambda>(t\<^sub>1, t\<^sub>2). t\<^sub>1 \<approx> t\<^sub>2) ` I"
+
+    assume "trans I" and "sym I" and "?I' \<TTurnstile> P"
+    then obtain K :: "('f, 'v) Term.term uprod literal" where
+      "K \<in># P" and "?I' \<TTurnstile>l K"
+      by (auto simp: true_cls_def)
+
+    show "?I' \<TTurnstile> C"
+    proof (cases "K = L\<^sub>1 \<or> K = L\<^sub>2")
+      case True
+      hence "I \<TTurnstile>l Pos (t\<^sub>2, s\<^sub>1') \<or> I \<TTurnstile>l Pos (t\<^sub>2, t\<^sub>2')"
+        unfolding eq_factoringI \<open>s\<^sub>1 = t\<^sub>2\<close>
+        using \<open>?I' \<TTurnstile>l K\<close> true_lit_uprod_iff_true_lit_prod[OF \<open>sym I\<close>] by metis
+      hence "I \<TTurnstile>l Pos (s\<^sub>1, t\<^sub>2') \<or> I \<TTurnstile>l Neg (s\<^sub>1', t\<^sub>2')"
+      proof (elim disjE)
+        assume "I \<TTurnstile>l Pos (t\<^sub>2, s\<^sub>1')"
+        then show ?thesis
+          unfolding \<open>s\<^sub>1 = t\<^sub>2\<close> true_lit_simps
+          by (metis \<open>trans I\<close> transD)
+      next
+        assume "I \<TTurnstile>l Pos (t\<^sub>2, t\<^sub>2')"
+        then show ?thesis
+          using \<open>s\<^sub>1 = t\<^sub>2\<close> by simp
+      qed
+      hence "?I' \<TTurnstile>l Pos (s\<^sub>1 \<approx> t\<^sub>2') \<or> ?I' \<TTurnstile>l Neg (s\<^sub>1' \<approx> t\<^sub>2')"
+        unfolding true_lit_uprod_iff_true_lit_prod[OF \<open>sym I\<close>] .
+      hence "?I' \<TTurnstile>l Pos (s\<^sub>1 \<approx> t\<^sub>2') \<cdot>l \<mu> \<or> ?I' \<TTurnstile>l Neg (s\<^sub>1' \<approx> t\<^sub>2') \<cdot>l \<mu>"
+        using \<open>is_ground_atm (s\<^sub>1 \<approx> s\<^sub>1')\<close> \<open>is_ground_atm (t\<^sub>2 \<approx> t\<^sub>2')\<close> by auto
+      thus ?thesis
+        unfolding eq_factoringI
+        by (metis subst_cls_add_mset true_cls_add_mset)
+    next
+      case False
+      hence "K \<in># P'"
+        using \<open>K \<in># P\<close>
+        unfolding eq_factoringI
+        by auto
+      hence "K \<in># C"
+        using ground_P
+        by (simp add: eq_factoringI(1,2,3,7))
+      thus ?thesis
+        using \<open>(\<lambda>(t\<^sub>1, t\<^sub>2). t\<^sub>1 \<approx> t\<^sub>2) ` I \<TTurnstile>l K\<close> by blast
+    qed
+  qed
+qed
 
 interpretation G: sound_inference_system G_Inf G_Bot G_entails
 proof unfold_locales
+  show "G_Bot \<noteq> {}"
+    by simp
+next
+  show "\<And>B N. B \<in> G_Bot \<Longrightarrow> G_entails {B} N"
+    by (simp add: G_entails_def)
+next
+  show "\<And>N2 N1. N2 \<subseteq> N1 \<Longrightarrow> G_entails N1 N2"
+    by (auto simp: G_entails_def elim!: true_clss_mono[rotated])
+next
+  fix N1 N2 assume ball_G_entails: "\<forall>C \<in> N2. G_entails N1 {C}"
+  show "G_entails N1 N2"
+    unfolding G_entails_def
+  proof (intro allI impI)
+    fix I
+    assume "refl I" and "trans I" and "sym I" and "compatible_with_Fun I" and
+      "(\<lambda>(x, y). x \<approx> y) ` I \<TTurnstile>s cls_gcls ` N1"
+    hence "\<forall>C \<in> N2. (\<lambda>(x, y). x \<approx> y) ` I \<TTurnstile>s {cls_gcls C}"
+      using ball_G_entails by (simp add: G_entails_def)
+    then show "(\<lambda>(x, y). x \<approx> y) ` I \<TTurnstile>s cls_gcls ` N2"
+      by (simp add: true_clss_def)
+  qed
+next
+  show "\<And>N1 N2 N3. G_entails N1 N2 \<Longrightarrow> G_entails N2 N3 \<Longrightarrow> G_entails N1 N3"
+    using G_entails_def by simp
+next
   show "\<And>\<iota>. \<iota> \<in> G_Inf \<Longrightarrow> G_entails (set (prems_of \<iota>)) {concl_of \<iota>}"
-    sorry
+    unfolding G_Inf_def
+    using correctness_ground_superposition
+    using correctness_ground_eq_resolution
+    using correctness_ground_eq_factoring
+    by (auto simp: G_entails_def)
 qed
 
-interpretation G: calculus_with_finitary_standard_redundancy G_Inf G_Bot G_entails "(\<prec>\<^sub>c)"
+lemma smaller_conclusion_ground_eq_resolution:
+  assumes step: "eq_resolution P C" and ground_P: "is_ground_cls P"
+  shows "C \<prec>\<^sub>c P"
+  using step
+proof (cases P C rule: eq_resolution.cases)
+  case (eq_resolutionI L P' s\<^sub>1 s\<^sub>2 \<mu>)
+  then show ?thesis
+    using totalp_on_less_cls
+    by (metis add.right_neutral add_mset_add_single empty_iff empty_not_add_mset ground_P
+        one_step_implies_multp set_mset_empty subst_cls_ident_if_is_ground_cls sup_eq_bot_iff
+        vars_cls_add_mset)
+qed
+
+lemma smaller_conclusion_ground_eq_factoring:
+  assumes step: "eq_factoring P C" and ground_P: "is_ground_cls P"
+  shows "C \<prec>\<^sub>c P"
+  using step
+proof (cases P C rule: eq_factoring.cases)
+  case (eq_factoringI L\<^sub>1 L\<^sub>2 P' s\<^sub>1 s\<^sub>1' t\<^sub>2 t\<^sub>2' \<mu>)
+  with ground_P have
+    "is_ground_trm s\<^sub>1" and "is_ground_trm s\<^sub>1'" and "is_ground_trm t\<^sub>2" and "is_ground_trm t\<^sub>2'"
+    by simp_all
+  hence subst_ident: "s\<^sub>1 \<cdot>t \<sigma> = s\<^sub>1" "s\<^sub>1' \<cdot>t \<sigma> = s\<^sub>1'" "t\<^sub>2 \<cdot>t \<sigma> = t\<^sub>2" "t\<^sub>2' \<cdot>t \<sigma> = t\<^sub>2'" for \<sigma>
+    by simp_all
+
+  have "term_subst.is_unifier \<mu> {s\<^sub>1, t\<^sub>2}"
+    using \<open>term_subst.is_imgu \<mu> {{s\<^sub>1, t\<^sub>2}}\<close>
+    by (simp add: term_subst.is_imgu_def term_subst.is_unifiers_def)
+  moreover have "term_subst.is_ground_set {s\<^sub>1, t\<^sub>2}"
+    using \<open>is_ground_trm s\<^sub>1\<close> \<open>is_ground_trm t\<^sub>2\<close>
+    by (simp add: term_subst.is_ground_set_def term_subst.is_ground_def)
+  ultimately have "s\<^sub>1 = t\<^sub>2"
+    using term_subst.ball_eq_constant_if_unifier[of "{_}", simplified] by auto
+  hence "s\<^sub>1' \<prec>\<^sub>t t\<^sub>2"
+    using \<open>\<not> s\<^sub>1 \<cdot>t \<mu> \<preceq>\<^sub>t s\<^sub>1' \<cdot>t \<mu>\<close> \<open>is_ground_trm s\<^sub>1\<close> \<open>is_ground_trm s\<^sub>1'\<close>
+    using totalp_on_less_trm[THEN totalp_onD, unfolded mem_Collect_eq]
+    by (auto simp: subst_ident)
+
+  have "is_ground_atm (s\<^sub>1 \<approx> s\<^sub>1')"
+    by (simp add: \<open>is_ground_trm s\<^sub>1'\<close> \<open>is_ground_trm s\<^sub>1\<close>)
+
+  have "is_ground_atm (t\<^sub>2 \<approx> t\<^sub>2')"
+    by (simp add: \<open>is_ground_trm t\<^sub>2'\<close> \<open>is_ground_trm t\<^sub>2\<close>)
+
+  have "is_maximal_lit (L\<^sub>1 \<cdot>l \<mu>) (P \<cdot> \<mu>)"
+    using eq_factoringI by simp
+  hence "is_maximal_lit L\<^sub>1 P"
+    using ground_P eq_factoringI(1) by force
+  hence "\<forall>K \<in># add_mset (Pos (t\<^sub>2 \<approx> t\<^sub>2')) P'. \<not> Pos (s\<^sub>1 \<approx> s\<^sub>1') \<prec>\<^sub>l K"
+    unfolding eq_factoringI
+    by (simp add: is_maximal_wrt_def)
+  hence "\<not> Pos (s\<^sub>1 \<approx> s\<^sub>1') \<prec>\<^sub>l Pos (t\<^sub>2 \<approx> t\<^sub>2')"
+    by simp
+  hence "(t\<^sub>2 \<approx> t\<^sub>2') \<preceq>\<^sub>a (s\<^sub>1 \<approx> s\<^sub>1')"
+    using totalp_on_less_atm[THEN totalp_onD, unfolded mem_Collect_eq,
+        OF \<open>is_ground_atm (s\<^sub>1 \<approx> s\<^sub>1')\<close> \<open>is_ground_atm (t\<^sub>2 \<approx> t\<^sub>2')\<close>]
+    by force
+  hence "t\<^sub>2' \<preceq>\<^sub>t s\<^sub>1'"
+    unfolding \<open>s\<^sub>1 = t\<^sub>2\<close>
+    unfolding reflclp_iff
+    apply (simp add: make_uprod_eq_make_uprod_sym_iff)
+    apply safe
+    unfolding multp_cancel_add_mset[OF transp_less_trm
+        irreflp_on_subset[OF irreflp_less_trm subset_UNIV]]
+    by (smt (verit, del_insts) multp_implies_one_step set_mset_add_mset_insert set_mset_empty
+        single_is_union singletonD transp_less_trm union_single_eq_member)
+
+  from eq_factoringI have "C = add_mset (Pos (s\<^sub>1 \<approx> t\<^sub>2')) (add_mset (Neg (s\<^sub>1' \<approx> t\<^sub>2')) P')"
+    using ground_P by auto
+
+  moreover have "add_mset (Neg (s\<^sub>1' \<approx> t\<^sub>2')) (add_mset (Pos (s\<^sub>1 \<approx> t\<^sub>2')) P') \<prec>\<^sub>c P"
+    unfolding eq_factoringI \<open>s\<^sub>1 = t\<^sub>2\<close>
+  proof (intro one_step_implies_multp[of "{#_#}" "{#_#}", simplified])
+    have "t\<^sub>2' \<prec>\<^sub>t t\<^sub>2"
+      using \<open>s\<^sub>1' \<prec>\<^sub>t t\<^sub>2\<close> \<open>t\<^sub>2' \<preceq>\<^sub>t s\<^sub>1'\<close>
+      by (metis reflclp_iff transpD transp_less_trm)
+    thus "Neg (s\<^sub>1' \<approx> t\<^sub>2') \<prec>\<^sub>l Pos (t\<^sub>2 \<approx> s\<^sub>1')"
+      apply simp
+      by (smt (verit) add_mset_add_single add_mset_commute multi_self_add_other_not_self
+          one_step_implies_multp set_mset_add_mset_insert set_mset_empty singletonD
+          union_single_eq_member)
+  qed
+
+  ultimately show ?thesis
+    unfolding eq_factoringI
+    by (simp add: add_mset_commute)
+qed
+
+interpretation G: calculus_with_finitary_standard_redundancy G_Inf G_Bot G_entails
+  "\<lambda>C\<^sub>1 C\<^sub>2. cls_gcls C\<^sub>1 \<prec>\<^sub>c cls_gcls C\<^sub>2"
 proof unfold_locales
-  have "transp (\<prec>\<^sub>a)"
-    using transp_less_trm transp_lex_prodp by blast
-  hence "transp (\<prec>\<^sub>l)"
-    using transp_less_lit by blast
-  thus "transp (\<prec>\<^sub>c)"
-    using transp_multp by blast
+  show "transp (\<lambda>C\<^sub>1 C\<^sub>2. cls_gcls C\<^sub>1 \<prec>\<^sub>c cls_gcls C\<^sub>2)"
+    using transp_less_cls
+    by (metis (no_types, lifting) transpD transpI)
 next
   have "wfP (\<prec>\<^sub>a)"
-    using wfP_less_trm wfP_lex_prodp by blast
+    using wfP_less_trm wfP_multp
+    by (metis (no_types, lifting) wfP_if_convertible_to_wfP)
   hence "wfP (\<prec>\<^sub>l)"
     using wfP_less_lit by blast
-  thus "wfP (\<prec>\<^sub>c)"
+  hence "wfP (\<prec>\<^sub>c)"
     using wfP_multp by blast
+  thus "wfP (\<lambda>C\<^sub>1 C\<^sub>2. cls_gcls C\<^sub>1 \<prec>\<^sub>c cls_gcls C\<^sub>2)"
+    by (metis (no_types, lifting) wfP_if_convertible_to_wfP)
 next
   show "\<And>\<iota>. \<iota> \<in> G_Inf \<Longrightarrow> prems_of \<iota> \<noteq> []"
-    sorry
+    by (auto simp: G_Inf_def)
 next
-  show "\<And>\<iota>. \<iota> \<in> G_Inf \<Longrightarrow> concl_of \<iota> \<prec>\<^sub>c main_prem_of \<iota>"
+  show "\<And>\<iota>. \<iota> \<in> G_Inf \<Longrightarrow> cls_gcls (concl_of \<iota>) \<prec>\<^sub>c cls_gcls (main_prem_of \<iota>)"
     sorry
 qed
 
@@ -317,24 +793,24 @@ qed
 section \<open>First-Order Layer\<close>
 
 
-abbreviation F_Inf :: "('f, 'v) atom clause inference set" where
+abbreviation F_Inf :: "('f, 'v) term atom clause inference set" where
   "F_Inf \<equiv> {}"
 
-abbreviation F_Bot :: "('f, 'v) atom clause set" where
+abbreviation F_Bot :: "('f, 'v) term atom clause set" where
   "F_Bot \<equiv> {{#}}"
 
-abbreviation F_entails :: "('f, 'v) atom clause set \<Rightarrow> ('f, 'v) atom clause set \<Rightarrow> bool" where
+abbreviation F_entails :: "('f, 'v) term atom clause set \<Rightarrow> ('f, 'v) term atom clause set \<Rightarrow> bool" where
   "F_entails \<equiv> (\<TTurnstile>e)"
 
 typedecl Q
 
-definition \<G>_F :: "Q \<Rightarrow> ('f, 'v) atom clause \<Rightarrow> ('f, 'v) atom clause set" where
+definition \<G>_F :: "Q \<Rightarrow> ('f, 'v) term atom clause \<Rightarrow> ('f, 'v) term atom clause set" where
   "\<G>_F \<equiv> \<lambda>_ _. {}"
 
-definition \<G>_I :: "Q \<Rightarrow> ('f, 'v) atom clause inference \<Rightarrow> ('f, 'v) atom clause inference set option" where
+definition \<G>_I :: "Q \<Rightarrow> ('f, 'v) term atom clause inference \<Rightarrow> ('f, 'v) term atom clause inference set option" where
   "\<G>_I \<equiv> \<lambda>_ _. None"
 
-definition Prec_F :: "('f, 'v) atom clause \<Rightarrow> ('f, 'v) atom clause \<Rightarrow> ('f, 'v) atom clause \<Rightarrow> bool" where
+definition Prec_F :: "('f, 'v) term atom clause \<Rightarrow> ('f, 'v) term atom clause \<Rightarrow> ('f, 'v) term atom clause \<Rightarrow> bool" where
   "Prec_F \<equiv> \<lambda>_ _ _. False"
 
 interpretation F: lifting_intersection F_Inf G_Bot "UNIV :: Q set" "\<lambda>(_ :: Q). G_Inf"
