Superposition_Calculus/Multiset_Extra.thy
@@ -1,0 +1,8 @@
+theory Multiset_Extra
+  imports "HOL-Library.Multiset"
+begin
+  
+definition is_maximal_wrt where
+  "is_maximal_wrt R x M \<longleftrightarrow> (\<forall>y \<in># M - {#x#}. \<not> (R x y))"
+
+end
